theories/vir/mcfg_contextual_proof.v
@@ -1,0 +1,1502 @@
+From iris.prelude Require Import options.
+
+From Coq Require Import Program.Equality.
+
+From velliris.program_logic Require Import program_logic.
+From velliris.vir Require Import
+  vir val_rel heapbij adequacy spec globalbij logical_relations fundamental
+  interp_properties.
+
+From Vellvm Require Import Syntax.DynamicTypes Handlers Syntax.LLVMAst
+  Semantics.InterpretationStack.
+
+From Equations Require Import Equations.
+
+From ITree Require Import
+  ITree Recursion Eq.Eqit Events.StateFacts Interp.InterpFacts.
+From Equations Require Import Equations.
+
+Set Default Proof Using "Type*".
+
+Import LLVMEvents.
+(* -------------------------------------------------------------------------- *)
+
+(* ITree-related tactics *)
+Ltac obs_hyp :=
+  match goal with
+  | [ H : {| _observe := observe _ |} = _ |- _] =>
+      let Hobs := fresh "Hobs" in
+      inversion H as [ Hobs ]; clear H
+  end.
+
+(* Turn an [observe] hypothesis to an ITree equivalence. *)
+Ltac simpobs_eqit :=
+  try obs_hyp;
+  match goal with
+  | [ H : observe _ = _ |- _] =>
+      symmetry in H; apply Eqit.simpobs in H
+  end.
+
+(** *Top-level Contextual Refinement *)
+Section CR.
+
+  Context {Σ} `{!sheapGS Σ, !checkedoutGS Σ, !heapbijGS Σ}.
+
+  Definition globals_WF (g : vir.globals) : iPropI Σ :=
+    ([∗ map] g0↦v ∈ g, ∃ v' : dvalue, ⌜g !! g0 = Some v'⌝ ∗ dval_rel v' v)%I.
+
+  Definition mcfg_fn_disjoint_keys (C : CFG.mcfg dtyp) e :=
+     forall c, Leaf.Leaf c (mcfg_definitions C) -> disjoint_keys c e.
+
+  Definition lift_eutt_post {E} {R1 R2}
+    (Φ: R1 → R2 → iProp Σ) :=
+    (λ (e_t : itree E R1) (e_s : itree E R2), ∃ v_t v_s, ⌜e_t ≈ Ret v_t⌝ ∗ ⌜e_s ≈ Ret v_s⌝ ∗ Φ v_t v_s)%I.
+
+  (* Relating results on the hole. *)
+  Definition logrel_eutt_post : expr vir_lang uvalue → expr vir_lang uvalue → iPropI Σ :=
+    lift_eutt_post uval_rel.
+
+  #[global] Instance Proper_eutt_lift_eutt_post {E R1 R2} (Φ: R1 → R2 → iProp Σ) :
+    Proper (eutt eq ==> eutt (E := E) eq ==> equiv) (lift_eutt_post Φ).
+  Proof.
+    repeat intro; iSplit; iIntros "H";
+      rewrite /lift_eutt_post; iDestruct "H" as (????) "H";
+      repeat iExists _; repeat iSplitL ""; try iPureIntro; auto.
+    all : try rewrite -H1;try rewrite -H2; auto; symmetry; auto.
+  Qed.
+
+  Notation st_expr_rel' R1 R2 :=
+    (@st_exprO' vir_lang R1 -d> @st_exprO' vir_lang R2 -d> iPropI Σ).
+
+  (* An obligation for each of the defined calls; it satisfies the external
+      call specifications *)
+  Definition context_rel_call_inv
+      (f : ∀ T : Type, CallE T → L0'expr T)
+      (g : ∀ T : Type, CallE T → L0'expr T) :=
+    (□ (∀ fn1 fn2 dt1 dt2 attr1 attr2 args1 args2 C,
+          let call1 := ExternalCall dt1 fn1 args1 attr1 in
+          let call2 := ExternalCall dt2 fn2 args2 attr2 in
+          call_ev call1 call2 C -∗
+          ⟅ f _ (Call dt1 fn1 args1 attr1) ⟆ ⪯
+          ⟅ g _ (Call dt2 fn2 args2 attr2) ⟆
+          [[ (fun v1 v2 => call_ans call1 v1 call2 v2 C) ⤉ ]]) )%I.
+
+  (* Should follow by reflexivity theorem *)
+  Definition context_rel_refl
+      (f : ∀ T : Type, CallE T → L0'expr T)
+      (g : ∀ T : Type, CallE T → L0'expr T) :=
+    (□ (∀ fn1 fn2 dt attr args1 args2 C,
+          arg_val_rel (fn1, args1) (fn2, args2) C -∗
+          ⟅ f _ (Call dt fn1 args1 attr) ⟆ ⪯
+          ⟅ g _ (Call dt fn2 args2 attr) ⟆
+          [[ (fun x y => res_val_rel x y C) ⤉ ]]))%I.
+
+  (* Definition context_call *)
+  (*     (f : ∀ T : Type, CallE T → L0'expr T) := *)
+  (*   (forall τ addr args attrs, *)
+  (*     f uvalue (Call τ addr args attrs) = *)
+  (*     f uvalue (ExternalCall τ addr args attrs)). *)
+  (*   (forall τ addr args attrs, *)
+  (*     f uvalue (Call τ addr args (FNATTR_External:: attrs)) = *)
+  (*     f uvalue (Call τ addr args attrs)). *)
+
+
+
+  Definition context_rel
+      (f : ∀ T : Type, CallE T → L0'expr T)
+      (g : ∀ T : Type, CallE T → L0'expr T) :=
+    (context_rel_call_inv f g ∗ context_rel_refl f g)%I.
+
+  (* Auxiliary definitions for [Proper_interp_mrec] *)
+  (* Because [sim_expr] includes stateful interpretation, showing properness result
+    for [interp_mrec] amounts to proving a simulation *)
+  Local Definition interp_mrec_pred {R1 R2} :=
+    fun (Φ:st_expr_rel' R1 R2) (e_t:st_expr' vir_lang R1) (e_s:st_expr' vir_lang R2) =>
+      (∃ f a1 σ_t g a2 σ_s,
+          ⌜e_t = observe (⟦ interp_mrec f a1 ⟧ σ_t)⌝ ∗
+          ⌜e_s = observe (⟦ interp_mrec g a2 ⟧ σ_s)⌝ ∗
+         □ (∀ x y, (base x y ∗ Φ x y) ∗-∗ Φ x y) ∗
+         context_rel f g ∗
+         sim_coindF Φ (observe (⟦ ⟅ a1 ⟆ ⟧ σ_t)) (observe (⟦ ⟅ a2 ⟆ ⟧ σ_s)))%I.
+
+  Local Definition interp_mrec_rec {R1 R2} :=
+    fun (Φ:st_expr_rel' R1 R2) (e_t:st_expr' vir_lang R1) (e_s:st_expr' vir_lang R2) =>
+      ((∃ f a1 σ_t g a2 σ_s,
+          ⌜e_t = observe (⟦ interp_mrec f a1 ⟧ σ_t)⌝ ∗
+          ⌜e_s = observe (⟦ interp_mrec g a2 ⟧ σ_s)⌝ ∗
+         □ (∀ x y, (base x y ∗ Φ x y) ∗-∗ Φ x y) ∗
+         context_rel f g ∗
+          sim_coindF Φ (observe (⟦ ⟅ a1 ⟆ ⟧ σ_t)) (observe (⟦ ⟅ a2 ⟆ ⟧ σ_s)))
+        ∨ sim_coindF Φ e_t e_s)%I.
+
+  Local Instance interp_mrec_pred_ne {R1 R2}:
+    NonExpansive (interp_mrec_pred: st_expr_rel' R1 R2 -d> st_expr_rel' R1 R2).
+  Proof.
+    intros x y * H. solve_proper_prepare. do 18 f_equiv; try solve_proper.
+  Qed.
+
+  Local Instance interp_mrec_rec_ne {R1 R2}:
+    NonExpansive (interp_mrec_rec: st_expr_rel' R1 R2 -d> st_expr_rel' R1 R2).
+  Proof.
+    intros x y * H. solve_proper_prepare. repeat f_equiv; try solve_proper.
+  Qed.
+
+  Local Definition interp_mrec_ind {T} :=
+    (λ Φ e_t e_s,
+      ∀ (f g : ∀ T : Type, LLVMEvents.CallE T → L0'expr T)
+        (a1 a2 : itree (CallE +' language.L0 vir_lang) T) σ_t σ_s,
+      □ (∀ x y, (base x y ∗ Φ x y) ∗-∗ Φ x y) -∗
+      ⌜e_t = observe (⟦ ⟅ a1 ⟆ ⟧ σ_t) ⌝ -∗
+      ⌜e_s = observe (⟦ ⟅ a2 ⟆ ⟧ σ_s) ⌝ -∗
+      context_rel f g -∗
+      sim_indF interp_mrec_rec Φ
+          (observe (⟦ interp_mrec f a1 ⟧ σ_t))
+          (observe (⟦ interp_mrec g a2 ⟧ σ_s)))%I.
+
+  Local Instance interp_mrec_ind_ne {T}:
+    NonExpansive (interp_mrec_ind: st_expr_rel' _ _ -d> st_expr_rel' _ T).
+  Proof.
+    solve_proper_prepare. clear -H. repeat f_equiv. done.
+  Qed.
+
+  Lemma interp_mrec_F_ind_case {T}
+    (f g : ∀ T : Type, LLVMEvents.CallE T → L0'expr T) Ψ
+    t X (e : _ X) k σ_s σ_t (a1 a2 : _ T):
+    a1 ≅ vis e k ->
+    t ≅ vis (e : language.F _ _) (λ x, Tau (Tau (⟦ ⟅ k x ⟆ ⟧ σ_t))) ->
+    □ (∀ x y, (base x y ∗ Ψ x y) ∗-∗ Ψ x y) -∗
+    context_rel f g -∗
+    interp_mrec_ind Ψ (observe t) (observe (⟦ ⟅ a2 ⟆ ⟧ σ_s))
+              ∧ sim_indF sim_coindF Ψ (observe t) (observe (⟦ ⟅ a2 ⟆ ⟧ σ_s)) -∗
+    sim_expr_inner interp_mrec_rec (sim_indF interp_mrec_rec) Ψ
+      (observe (⟦ interp_mrec f a1 ⟧ σ_t))
+      (observe (⟦ interp_mrec g a2 ⟧ σ_s)).
+  Proof.
+    intros Ha Ht.
+    to_eq in Ht; rewrite Ht; clear Ht.
+    to_eq in Ha; rewrite Ha; clear Ha.
+
+    iIntros "#HΨ Hfg Hinner".
+    iDestruct "Hinner" as "(_ & Hinner)".
+    rewrite -sim_coindF_unfold. rewrite /sim_expr_inner.
+    iPoseProof (sim_coindF_F_inv_L with "HΨ Hinner") as ">Hinner".
+
+    change
+      (|==>
+        ∃ c : sim_case,
+          match c with
+          | BASE => _
+          | STUTTER_L => stutter_l
+          | STUTTER_R => stutter_r
+          | TAU_STEP => tau_step
+          | VIS_STEP => _
+          | SOURCE_UB => source_ub
+          | SOURCE_EXC => source_exc
+          end)%I with
+          (sim_expr_inner interp_mrec_rec (sim_indF interp_mrec_rec) Ψ
+            (observe (⟦ interp_mrec f (vis e k) ⟧ σ_t))
+            (observe (⟦ interp_mrec g a2 ⟧ σ_s))).
+
+    iDestruct "Hinner" as "[ Hinner | [ Hinner | Hinner ] ]".
+    { iDestruct "Hinner" as (???) "Hinner".
+      rewrite -itree_eta in H.
+      apply interp_L2_conv_F_tau_n_inv with (g := g) in H.
+      destruct H as (?&?&?&?&?).
+      to_eq in H0; rewrite H0 -sim_indF_unfold.
+      rewrite interp_mrec_vis.
+      iApply sim_indF_n_taus_R.
+      rewrite sim_indF_unfold; provide_case: STUTTER_L.
+      cbn. rewrite sim_indF_unfold; provide_case: VIS_STEP.
+      rewrite /handle_event; cbn; rewrite /handle_E.
+      iSplitL ""; first (iPureIntro; by exists eq_refl).
+      iIntros. dependent destruction H1; cbn.
+      change (TauF ?x) with (observe (Tau x)).
+      rewrite -!interp_mrec_tau.
+      iLeft; iModIntro.
+      iExists f, _, _, g, _, _; iFrame.
+      repeat (iSplitL ""; first done).
+      rewrite !interp_L2_conv_tau.
+      specialize (H v_s); to_eq in H; rewrite -H.
+      by do 2 iApply sim_coindF_tauL. }
+
+    { iDestruct "Hinner" as (?????) "Hinner".
+      rewrite -itree_eta in H.
+      eapply interp_L2_conv_UB_tau_n_inv with (g := g) in H.
+      destruct H as (?&?).
+      to_eq in H; rewrite H.
+      rewrite -sim_indF_unfold; iApply sim_indF_n_taus_R.
+      rewrite sim_indF_unfold; by provide_case: SOURCE_UB. }
+
+    { iDestruct "Hinner" as (?????) "Hinner".
+      rewrite -itree_eta in H.
+      eapply interp_L2_conv_failure_tau_n_inv with (g := g) in H.
+      destruct H as (?&?&?).
+      to_eq in H; rewrite H.
+      rewrite -sim_indF_unfold; iApply sim_indF_n_taus_R.
+      rewrite sim_indF_unfold; by provide_case: SOURCE_EXC.
+      Unshelve. all : eauto. }
+  Qed.
+
+  Lemma interp_mrec_F_ind_case' {T}
+    (f g : ∀ T : Type, LLVMEvents.CallE T → L0'expr T) Ψ
+    t X (e : _ X) k σ_s σ_t (a1 a2 : _ T):
+    a2 ≅ vis e k ->
+    t ≅ vis (e : language.F _ _) (λ x, Tau (Tau (⟦ ⟅ k x ⟆ ⟧ σ_s))) ->
+    □ (∀ x y, (base x y ∗ Ψ x y) ∗-∗ Ψ x y) -∗
+    context_rel f g -∗
+    interp_mrec_ind Ψ (observe (⟦ ⟅ a1 ⟆ ⟧ σ_t)) (observe t) 
+              ∧ sim_indF sim_coindF Ψ (observe (⟦ ⟅ a1 ⟆ ⟧ σ_t)) (observe t) -∗
+    sim_expr_inner interp_mrec_rec (sim_indF interp_mrec_rec) Ψ
+      (observe (⟦ interp_mrec f a1 ⟧ σ_t)) (observe (⟦ interp_mrec g a2 ⟧ σ_s)).
+  Proof.
+    intros Ha Ht.
+    to_eq in Ht; rewrite Ht; clear Ht.
+    to_eq in Ha; rewrite Ha; clear Ha.
+
+    iIntros "#HΨ Hfg Hinner".
+    iDestruct "Hinner" as "(_ & Hinner)".
+    rewrite -sim_coindF_unfold. rewrite /sim_expr_inner.
+    iPoseProof (sim_coindF_F_inv_R with "HΨ Hinner") as ">Hinner".
+
+    change
+      (|==>
+        ∃ c : sim_case,
+          match c with
+          | BASE => _
+          | STUTTER_L => stutter_l
+          | STUTTER_R => stutter_r
+          | TAU_STEP => tau_step
+          | VIS_STEP => _
+          | SOURCE_UB => source_ub
+          | SOURCE_EXC => source_exc
+          end)%I with
+          (sim_expr_inner interp_mrec_rec (sim_indF interp_mrec_rec) Ψ
+            (observe (⟦ interp_mrec f a1 ⟧ σ_t))
+            (observe (⟦ interp_mrec g (vis e k) ⟧ σ_s))).
+
+    iDestruct "Hinner" as (???) "Hinner".
+    rewrite -itree_eta in H.
+    apply interp_L2_conv_F_tau_n_inv with (g := f) in H.
+    destruct H as (?&?&?&?&?).
+    to_eq in H0; rewrite H0 -sim_indF_unfold.
+    rewrite interp_mrec_vis.
+    iApply sim_indF_n_taus_L.
+    rewrite sim_indF_unfold; provide_case: STUTTER_R.
+    cbn. rewrite sim_indF_unfold; provide_case: VIS_STEP.
+    rewrite /handle_event; cbn; rewrite /handle_E.
+    iSplitL ""; first (iPureIntro; by exists eq_refl).
+    iIntros. dependent destruction H1; cbn.
+    change (TauF ?x) with (observe (Tau x)).
+    rewrite -!interp_mrec_tau.
+    iLeft; iModIntro.
+    iExists f, _, _, g, _, _; iFrame.
+    repeat (iSplitL ""; first done).
+    rewrite !interp_L2_conv_tau.
+    specialize (H v_s); to_eq in H; rewrite -H.
+    by do 2 iApply sim_coindF_tauR.
+  Qed.
+
+  Require Import LLVMEvents.
+
+  Lemma interp_mrec_failure_ind_case {T}
+    (f g : ∀ T : Type, LLVMEvents.CallE T → L0'expr T) Ψ
+    t X (e : _ X) k σ_s σ_t (a1 a2: _ T) :
+    t ≅ vis (e : FailureE _) k ->
+    □ (∀ x y, (base x y ∗ Ψ x y) ∗-∗ Ψ x y) -∗
+    interp_mrec_ind Ψ (observe t) (observe (⟦ ⟅ a2 ⟆ ⟧ σ_s))
+              ∧ sim_indF sim_coindF Ψ (observe t) (observe (⟦ ⟅ a2 ⟆ ⟧ σ_s)) -∗
+    sim_expr_inner interp_mrec_rec (sim_indF interp_mrec_rec) Ψ
+      (observe (⟦ interp_mrec f a1 ⟧ σ_t)) (observe (⟦ interp_mrec g a2 ⟧ σ_s)).
+  Proof.
+    intros H.
+    to_eq in H; rewrite H; clear H.
+    iIntros "#HΨ Hinner".
+    iDestruct "Hinner" as "(_ & Hinner)".
+    rewrite -sim_coindF_unfold.
+    iPoseProof (sim_coindF_fail_inv with "HΨ Hinner") as "%H'".
+
+    destruct H' as [ (?&?&?) | (?&?&?) ].
+    (* exception case *)
+    { eapply interp_L2_conv_failure_tau_n_inv in H.
+      destruct H as (?&?&?).
+      to_eq in H; rewrite H -sim_indF_unfold.
+      iApply sim_indF_n_taus_R.
+      rewrite sim_indF_unfold /sim_expr_inner.
+      by provide_case: SOURCE_EXC. }
+
+    (* UB case *)
+    { eapply interp_L2_conv_UB_tau_n_inv with (g := g) in H.
+      destruct H as (?&?); to_eq in H; rewrite H -sim_indF_unfold.
+      iApply sim_indF_n_taus_R; rewrite sim_indF_unfold.
+      by provide_case: SOURCE_UB. }
+
+    Unshelve. all : done.
+  Qed.
+
+  Lemma interp_mrec_UB_ind_case {T}
+    (f g : ∀ T : Type, LLVMEvents.CallE T → L0'expr T) Ψ
+    t X (e : _ X) k σ_s σ_t (a1 a2: _ T):
+    t ≅ vis (e : UBE _) k ->
+    □ (∀ x y, (base x y ∗ Ψ x y) ∗-∗ Ψ x y) -∗
+    interp_mrec_ind Ψ (observe t) (observe (⟦ ⟅ a2 ⟆ ⟧ σ_s))
+              ∧ sim_indF sim_coindF Ψ (observe t) (observe (⟦ ⟅ a2 ⟆ ⟧ σ_s)) -∗
+    sim_expr_inner interp_mrec_rec (sim_indF interp_mrec_rec) Ψ
+      (observe (⟦ interp_mrec f a1 ⟧ σ_t)) (observe (⟦ interp_mrec g a2 ⟧ σ_s)).
+  Proof.
+    intros H.
+    to_eq in H; rewrite H; clear H.
+    iIntros "HΨ Hinner".
+    iDestruct "Hinner" as "(_ & Hinner)".
+    rewrite -sim_coindF_unfold.
+    iPoseProof (sim_coindF_UBE_inv with "HΨ Hinner") as "%H'".
+
+    destruct H' as [ (?&?&?) | (?&?&?) ].
+    (* exception case *)
+    { eapply interp_L2_conv_failure_tau_n_inv in H.
+      destruct H as (?&?&?).
+      to_eq in H; rewrite H -sim_indF_unfold.
+      iApply sim_indF_n_taus_R.
+      rewrite sim_indF_unfold /sim_expr_inner.
+      by provide_case: SOURCE_EXC. }
+
+    (* UB case *)
+    { eapply interp_L2_conv_UB_tau_n_inv with (g := g) in H.
+      destruct H as (?&?).
+      to_eq in H; rewrite H -sim_indF_unfold.
+      iApply sim_indF_n_taus_R.
+      rewrite sim_indF_unfold /sim_expr_inner.
+      by provide_case: SOURCE_UB. }
+
+    Unshelve. all : done.
+  Qed.
+
+  Lemma interp_mrec_pred_coind_init {T}
+      (f : ∀ T : Type, CallE T → L0'expr T)
+      (g : ∀ T : Type, CallE T → L0'expr T)
+      (a1 a2 : itree L0' _) (σ_t σ_s : state vir_lang) Ψ:
+      context_rel f g -∗
+      ⟅ a1 ⟆ ⪯⟅ a2 ⟆ [[ Ψ ⤉ ]] -∗
+      state_interp σ_t σ_s ==∗
+      interp_mrec_pred (lift_rel (Ψ ⤉))
+        (observe (⟦ interp_mrec (T := T) f a1 ⟧ σ_t))
+        (observe (⟦ interp_mrec (T := T) g a2 ⟧ σ_s)).
+  Proof.
+    iIntros "H H' SI".
+    rewrite /interp_mrec_pred.
+    iExists f, a1, σ_t, g, a2, σ_s.
+    iMod ("H'" with "SI").
+    iModIntro.
+    do 2 (iSplitL ""; [ done | ]).
+    iSplitL ""; [ | iFrame ].
+    iIntros (??); iModIntro; iSplitL.
+    - iIntros "(H1 & H2)"; eauto.
+    - iIntros "H"; eauto.
+      iDestruct "H" as (????) "(SI & H)".
+      iDestruct "H" as (??) "H".
+      iDestruct "H" as (????) "H".
+      iSplitL "".
+      { rewrite /base. iExists _, _; eauto.
+        apply eqitree_inv_Ret_r in H1, H2.
+        cbn in H.
+        iSplit; iPureIntro.
+        { apply EqAxiom.bisimulation_is_eq.
+          rewrite H. rewrite -itree_eta.
+          rewrite (itree_eta e_t).
+          rewrite H1; cbn. rewrite /interp_L2.
+          setoid_rewrite StateFacts.interp_state_ret; done. }
+        { apply EqAxiom.bisimulation_is_eq.
+          rewrite H0. rewrite -itree_eta.
+          rewrite (itree_eta e_s).
+          rewrite H2; cbn. rewrite /interp_L2.
+          setoid_rewrite StateFacts.interp_state_ret; done. } }
+      { rewrite /base. iExists _, _; eauto.
+        apply eqitree_inv_Ret_r in H1, H2.
+        repeat iExists _; iFrame.
+        do 2 (iSplitL ""; [ done | ]).
+        repeat iExists _; iSplitL ""; try iPureIntro.
+        - setoid_rewrite (itree_eta e_t); by rewrite H1.
+        - setoid_rewrite (itree_eta e_s); rewrite H2; by iFrame "H". }
+  Qed.
+
+  Lemma Proper_interp_mrec_base_case {T}
+      (Ψ : st_exprO' T -d> st_exprO' T -d> iPropI Σ)
+      (a1 a2 : itree (CallE +' language.L0 vir_lang) T)
+      (f : ∀ T : Type, CallE T → L0'expr T)
+      (g : ∀ T : Type, CallE T → L0'expr T)
+      (σ_t σ_s : global_env * (local_env * lstack) * memory_stack) :
+    □ (∀ x y : st_exprO' T, base x y ∗ Ψ x y ∗-∗ Ψ x y) -∗
+    context_rel f g -∗
+    Ψ (observe (⟦ ⟅ a1 ⟆ ⟧ σ_t)) (observe (⟦ ⟅ a2 ⟆ ⟧ σ_s)) -∗
+    sim_expr_inner interp_mrec_rec (sim_indF interp_mrec_rec) Ψ
+      (observe (⟦ interp_mrec f a1 ⟧ σ_t)) (observe (⟦ interp_mrec g a2 ⟧ σ_s)).
+  Proof.
+    iIntros "#He Hinner Hr".
+    iSpecialize ("He" with "Hr").
+    iDestruct "He" as "(Hb & He)".
+    iDestruct "Hb" as (???) "%Hb".
+    inversion H; inversion Hb.
+    symmetry in H1; symmetry in H2.
+    apply simpobs, interp_L2_conv_ret_inv in H1, H2.
+    to_eq in H1; to_eq in H2; subst; cbn; by provide_case: BASE.
+  Qed.
+
+  Lemma Proper_interp_mrec_stutter_l_case {T}
+      (Ψ : st_exprO' T -d> st_exprO' T -d> iPropI Σ)
+      (f : ∀ T : Type, CallE T → L0'expr T)
+      (g : ∀ T : Type, CallE T → L0'expr T)
+      (a1 a2 : itree (CallE +' language.L0 vir_lang) T)
+      (σ_t σ_s : global_env * (local_env * lstack) * memory_stack)
+      (t : L2_expr vir_lang T)
+      (H0 : observe (⟦ ⟅ a1 ⟆ ⟧ σ_t) = TauF t) :
+    □ (∀ x y : st_exprO' T, base x y ∗ Ψ x y ∗-∗ Ψ x y) -∗
+    context_rel f g -∗
+    interp_mrec_ind Ψ (observe t) (observe (⟦ ⟅ a2 ⟆ ⟧ σ_s))
+    ∧ sim_indF sim_coindF Ψ (observe t) (observe (⟦ ⟅ a2 ⟆ ⟧ σ_s)) -∗
+    sim_expr_inner interp_mrec_rec (sim_indF interp_mrec_rec) Ψ
+      (observe (⟦ interp_mrec f a1 ⟧ σ_t)) (observe (⟦ interp_mrec g a2 ⟧ σ_s)).
+  Proof.
+    iIntros "He Hr Hinner".
+
+    symmetry in H0; apply simpobs in H0.
+    rewrite /sim_expr_inner.
+    apply interp_L2_conv_tau_inv in H0.
+    destruct H0 as [(?&?&?)| (?&?&?&?&?) ].
+    { (* Tau *)
+      iDestruct "Hinner" as "(Hinner & _)".
+      apply EqAxiom.bisimulation_is_eq in H0.
+      iSpecialize ("Hinner" $! f g _ _ _ _ with "He"); subst.
+      iSpecialize ("Hinner" $! eq_refl eq_refl with "Hr").
+      provide_case: STUTTER_L; symmetry in H.
+      apply simpobs, EqAxiom.bisimulation_is_eq in H; subst; cbn; by eauto. }
+
+    { (* Vis case *)
+      symmetry in H; apply simpobs in H.
+      to_eq in H; rewrite H.
+
+      pose proof (handle_noncall_L0_L2_case x x0 σ_t) as Hnoncall.
+      destruct Hnoncall as
+        [ (?&?) |
+          [ (?&?&?&?) |
+            [ (?&?&?&?) |
+              (?&?&?) ] ] ].
+
+      { (* [handle_noncall_L0_L2] Ret case *)
+        rewrite H1 bind_ret_l in H0.
+        iDestruct "Hinner" as "(Hinner & _)".
+        rewrite /F -!interp_state_tau -!interp_tau in H0; to_eq in H0; subst.
+        iSpecialize ("Hinner" $! f g (Tau (Tau (x1 x2.2)))
+                        _ x2.1 _ with "He").
+        iSpecialize ("Hinner" $! eq_refl eq_refl with "Hr").
+        to_eq in H1; rewrite interp_mrec_vis H1 !interp_mrec_tau.
+        by provide_case: STUTTER_L. }
+
+      { (* failure case *)
+        iApply (interp_mrec_failure_ind_case with "He Hinner"); eauto.
+        rewrite H0 H1; by tau_steps. }
+
+      { (* UB case *)
+        iApply (interp_mrec_UB_ind_case with "He Hinner"); eauto.
+        rewrite H0 H1; by tau_steps. }
+
+      { (* Other cases *)
+        dependent destruction H2.
+        iApply (interp_mrec_F_ind_case with "He Hr Hinner"); eauto.
+        { apply eqit_Vis; done. }
+
+        rewrite H0 H1 bind_vis. apply eqit_Vis.
+        intros. cbn. rewrite bind_ret_l. by cbn. } }
+  Qed.
+
+  Lemma Proper_interp_mrec_stutter_r_case {T}
+      (Ψ : st_exprO' T -d> st_exprO' T -d> iPropI Σ)
+      (f : ∀ T : Type, CallE T → L0'expr T)
+      (g : ∀ T : Type, CallE T → L0'expr T)
+      (a1 a2 : itree (CallE +' language.L0 vir_lang) T)
+      (σ_t σ_s : global_env * (local_env * lstack) * memory_stack)
+      (t : L2_expr vir_lang T)
+      (H0 : observe (⟦ ⟅ a2 ⟆ ⟧ σ_s) = TauF t):
+    □ (∀ x y : st_exprO' T, base x y ∗ Ψ x y ∗-∗ Ψ x y) -∗
+    context_rel f g -∗
+    interp_mrec_ind Ψ (observe (⟦ ⟅ a1 ⟆ ⟧ σ_t)) (observe t)
+    ∧ sim_indF sim_coindF Ψ (observe (⟦ ⟅ a1 ⟆ ⟧ σ_t)) (observe t) -∗
+    sim_expr_inner interp_mrec_rec (sim_indF interp_mrec_rec) Ψ
+      (observe (⟦ interp_mrec f a1 ⟧ σ_t))
+      (observe (⟦ interp_mrec g a2 ⟧ σ_s)).
+  Proof.
+    iIntros "He Hr Hinner".
+
+    symmetry in H0; apply simpobs in H0.
+    apply interp_L2_conv_tau_inv in H0.
+    destruct H0 as [(?&?&?)| (?&?&?&?&?) ].
+    { (* Tau *)
+      rewrite /sim_expr_inner.
+      iDestruct "Hinner" as "(Hinner & _)".
+      apply EqAxiom.bisimulation_is_eq in H0.
+      iSpecialize ("Hinner" $! f g _ _ _ _ with "He"); subst.
+      iSpecialize ("Hinner" $! eq_refl eq_refl with "Hr").
+      provide_case: STUTTER_R; symmetry in H.
+      apply simpobs, EqAxiom.bisimulation_is_eq in H; subst; cbn; by eauto. }
+
+    { (* Vis case *)
+      symmetry in H; apply simpobs in H.
+      to_eq in H; rewrite H.
+
+      pose proof (handle_noncall_L0_L2_case x x0 σ_s) as Hnoncall.
+      destruct Hnoncall as
+        [ (?&?) |
+          [ (?&?&?&?) |
+            [ (?&?&?&?) |
+              (?&?&?) ] ] ].
+
+      { (* [handle_noncall_L0_L2] Ret case *)
+        rewrite H1 bind_ret_l in H0.
+        iDestruct "Hinner" as "(Hinner & _)".
+        rewrite /F -!interp_state_tau -!interp_tau in H0; to_eq in H0; subst.
+        iSpecialize ("Hinner" $! f g _ _ _ _ with "He").
+        iSpecialize ("Hinner" $! eq_refl eq_refl with "Hr").
+        to_eq in H1; rewrite interp_mrec_vis H1 !interp_mrec_tau.
+        by provide_case: STUTTER_R. }
+
+      { (* failure case *)
+        iClear "Hinner". rewrite interp_mrec_vis; to_eq in H1; rewrite H1.
+        provide_case: STUTTER_R; cbn.
+        rewrite sim_indF_unfold. by provide_case: SOURCE_EXC. }
+
+      { (* UB case *)
+        iClear "Hinner". rewrite interp_mrec_vis; to_eq in H1; rewrite H1.
+        provide_case: STUTTER_R; cbn.
+        rewrite sim_indF_unfold. by provide_case: SOURCE_UB. }
+
+      { (* Other cases *)
+        dependent destruction H2.
+        iApply (interp_mrec_F_ind_case' with "He Hr Hinner"); eauto.
+        { apply eqit_Vis; done. }
+
+        rewrite H0 H1 bind_vis. apply eqit_Vis.
+        intros. cbn. rewrite bind_ret_l. by cbn. } }
+  Qed.
+
+  Lemma Proper_interp_mrec_tau_case {T}
+      (Ψ : st_exprO' T -d> st_exprO' T -d> iPropI Σ)
+      (f : ∀ T : Type, CallE T → L0'expr T)
+      (g : ∀ T : Type, CallE T → L0'expr T)
+      (a1 a2 : itree (CallE +' language.L0 vir_lang) T)
+      (σ_t σ_s : global_env * (local_env * lstack) * memory_stack)
+      (t s : L2_expr vir_lang T)
+      (H0 : observe (⟦ ⟅ a1 ⟆ ⟧ σ_t) = TauF t)
+      (H1 : observe (⟦ ⟅ a2 ⟆ ⟧ σ_s) = TauF s) :
+    □ (∀ x y : st_exprO' T, base x y ∗ Ψ x y ∗-∗ Ψ x y) -∗
+    context_rel f g -∗
+    sim_coindF Ψ (observe t) (observe s) -∗
+    sim_expr_inner interp_mrec_rec (sim_indF interp_mrec_rec) Ψ
+      (observe (⟦ interp_mrec f a1 ⟧ σ_t))
+      (observe (⟦ interp_mrec g a2 ⟧ σ_s)).
+  Proof.
+    iIntros "He Hr Hinner".
+    symmetry in H0, H1. apply simpobs in H0, H1.
+
+    apply interp_L2_conv_tau_inv in H0.
+    (* Target case analysis*)
+    destruct H0 as [(?&?&?)| (?&?&?&?&?)].
+
+    { (* Tau Tau *)
+      symmetry in H; apply simpobs in H; to_eq in H; subst.
+      rewrite interp_mrec_tau.
+
+      apply interp_L2_conv_tau_inv in H1.
+      destruct H1 as [(?&?&?)| (?&?&?&?&?) ].
+      - symmetry in H; apply simpobs in H; to_eq in H; subst.
+        rewrite interp_mrec_tau.
+        provide_case: TAU_STEP.
+        to_eq in H0; to_eq in H1; subst.
+        iLeft; iExists f, _, _, g, _, _;
+          do 2 (iSplitL ""; [ done | ]); by iFrame.
+
+      - symmetry in H; apply simpobs in H; to_eq in H; subst.
+        pose proof (handle_noncall_L0_L2_case x0 x1 σ_s).
+        destruct H as [ (?&?) | [ (?&?&?&?) | [ (?&?&?&?) | (?&?&?) ] ] ].
+        { rewrite interp_mrec_vis.
+          to_eq in H; rewrite H. rewrite H bind_ret_l in H1.
+          to_eq in H0; to_eq in H1; rewrite H0 H1.
+          provide_case: TAU_STEP.
+          iLeft.
+          iExists f, x, σ_t, g, (Tau (Tau (x2 x3.2))), x3.1.
+          (iSplitL ""; [ done | ]); iSplitL "".
+          { iPureIntro. f_equiv. to_eq. rewrite bind_ret_l.
+            by rewrite -!interp_mrec_tau. }
+          iFrame. by rewrite !interp_L2_conv_tau. }
+
+        { rewrite interp_mrec_vis.
+          to_eq in H; rewrite H. rewrite H bind_vis in H1.
+          to_eq in H0; to_eq in H1; rewrite H0 H1.
+          provide_case: TAU_STEP.
+          iRight; cbn. iClear "Hinner".
+          rewrite sim_coindF_unfold sim_indF_unfold.
+          rewrite /subevent; unfold_cat.
+          by provide_case: SOURCE_EXC. }
+
+        { rewrite interp_mrec_vis.
+          to_eq in H; rewrite H. rewrite H bind_vis in H1.
+          to_eq in H0; to_eq in H1; rewrite H0 H1.
+          provide_case: TAU_STEP.
+          iRight; cbn. iClear "Hinner".
+          rewrite sim_coindF_unfold sim_indF_unfold.
+          rewrite /subevent; unfold_cat.
+          by provide_case: SOURCE_UB. }
+
+        { rewrite interp_mrec_vis. iDestruct "He" as "#He".
+          to_eq in H; rewrite H. rewrite H bind_vis in H1.
+          setoid_rewrite bind_ret_l in H1.
+          to_eq in H0; to_eq in H1; rewrite H0 H1.
+          cbn; rewrite /subevent; unfold_cat.
+          iDestruct (sim_coindF_F_inv_R with "He Hinner") as ">H".
+          to_inner (interp_mrec_rec (R1 := T) (R2 := T)).
+          iDestruct "H" as (???) "H".
+          rewrite -itree_eta in H3.
+          pose proof (interp_L2_conv_F_tau_n_inv _ _ _ _ _ f H3) as H';
+            clear H3.
+          destruct H' as (?&?&?&?&?).
+          to_eq in H4. rewrite H4.
+          change (TauF (n_taus ?x ?n)) with (observe (n_taus x (S n))).
+          pose proof (n_taus_S (vis x3
+             (λ x7 : x0, Tau (Tau (⟦ interp_mrec f (x5 x7) ⟧ x6)))) x4).
+          to_eq in H5; rewrite -H5; clear H5.
+          rewrite -sim_indF_unfold; iApply sim_indF_n_taus_L.
+          rewrite sim_indF_unfold; provide_case: STUTTER_L.
+          rewrite sim_indF_unfold; provide_case: STUTTER_R.
+          rewrite sim_indF_unfold; provide_case: VIS_STEP.
+          iSplitL "".
+          { by iPureIntro; to_eq; rewrite -itree_eta bind_vis;
+            setoid_rewrite bind_ret_l; cbn. }
+
+          cbn; unfold_cat. rewrite /handle_E.
+          iSplitL ""; first (iPureIntro; by exists eq_refl).
+          iIntros. dependent destruction H5.
+          rewrite -!interp_mrec_tau.
+          iLeft; iExists f, _, _, g, _, _.
+          do 2 (iSplitL ""; [ done | ]); iSplitL ""; iFrame;
+          first done. rewrite !interp_L2_conv_tau.
+          do 2 iApply sim_coindF_tauR.
+          specialize (H3 v_s); to_eq in H3; rewrite -H3; by clear H3. } }
+
+    (* Event *)
+    symmetry in H; apply simpobs in H; to_eq in H; subst.
+    rewrite interp_mrec_vis.
+
+    pose proof (handle_noncall_L0_L2_case x x0 σ_t).
+    destruct H as [ (?&?) | [ (?&?&?&?) | [ (?&?&?&?) | (?&?&?) ] ] ].
+    { to_eq in H; rewrite H.
+      apply interp_L2_conv_tau_inv in H1.
+      destruct H1 as [(?&?&?)| (?&?&?&?&?) ].
+      - symmetry in H1; apply simpobs in H1; to_eq in H1; subst.
+        rewrite interp_mrec_tau.
+        provide_case: TAU_STEP.
+        iLeft; iExists f, _, _, g, _, _.
+        iSplitL "".
+        { iPureIntro. f_equiv. to_eq.
+          by rewrite bind_ret_l -!interp_mrec_tau. }
+          (iSplitL ""; [ done | ]); iFrame.
+        rewrite H bind_ret_l in H0.
+        to_eq in H2; to_eq in H0. rewrite -H2.
+        by rewrite !interp_L2_conv_tau -H0.
+
+      - symmetry in H1; apply simpobs in H1; to_eq in H1; subst.
+        pose proof (handle_noncall_L0_L2_case x3 x4 σ_s).
+        destruct H1 as [ (?&?) | [ (?&?&?&?) | [ (?&?&?&?) | (?&?&?) ] ] ].
+        { rewrite interp_mrec_vis.
+          to_eq in H1; rewrite H1.
+          provide_case: TAU_STEP.
+          iLeft. iExists f, _, _, g, _, _.
+
+          iSplitL "".
+          { iPureIntro. f_equiv. to_eq.
+            by rewrite bind_ret_l -!interp_mrec_tau. }
+          iSplitL "".
+          { iPureIntro. f_equiv. to_eq.
+            by rewrite bind_ret_l -!interp_mrec_tau. }
+          iFrame.
+          rewrite H bind_ret_l in H0. rewrite H1 bind_ret_l in H2.
+          to_eq in H2; to_eq in H0.
+          by rewrite !interp_L2_conv_tau -H0 -H2. }
+
+        { rewrite interp_mrec_vis.
+          to_eq in H1; rewrite H1.
+          provide_case: TAU_STEP.
+          iRight; cbn. iClear "Hinner".
+          rewrite sim_coindF_unfold sim_indF_unfold.
+          rewrite /subevent; unfold_cat.
+          by provide_case: SOURCE_EXC. }
+
+        { rewrite interp_mrec_vis.
+          to_eq in H1; rewrite H1.
+          provide_case: TAU_STEP.
+          iRight; cbn. iClear "Hinner".
+          rewrite sim_coindF_unfold sim_indF_unfold.
+          rewrite /subevent; unfold_cat.
+          by provide_case: SOURCE_UB. }
+
+        { rewrite interp_mrec_vis. iDestruct "He" as "#He".
+          to_eq in H1; rewrite H1. rewrite H1 bind_vis in H2.
+          setoid_rewrite bind_ret_l in H2.
+          rewrite H bind_ret_l in H0.
+          to_eq in H2; to_eq in H0; rewrite H2 H0.
+
+          iPoseProof (contains_base_tauL with "He") as "Ht".
+          do 2 iPoseProof (sim_coindF_TauL_inv with "Ht Hinner") as "Hinner".
+          iDestruct (sim_coindF_F_inv_R with "He Hinner") as ">H".
+          to_inner (interp_mrec_rec (R1 := T) (R2 := T)).
+          iDestruct "H" as (???) "H".
+          rewrite -itree_eta in H4.
+          provide_case: STUTTER_L; cbn.
+          rewrite sim_indF_unfold; provide_case: STUTTER_R.
+          do 2 (rewrite sim_indF_unfold; provide_case: STUTTER_L).
+          pose proof (interp_L2_conv_F_tau_n_inv _ _ _ _ _ f H4) as H';
+            clear H4.
+          destruct H' as (?&?&?&?&?).
+          to_eq in H5. rewrite H5.
+          iApply sim_indF_n_taus_L; cbn.
+          rewrite sim_indF_unfold; provide_case: VIS_STEP.
+          iSplitL "".
+          { iPureIntro; by exists eq_refl. }
+          iIntros (??) "%Hv". dependent destruction Hv; cbn.
+          change (TauF ?x) with (observe (Tau x)).
+          rewrite -!interp_mrec_tau.
+          iLeft; iExists f, _, _, g, _, _.
+          do 2 (iSplitL ""; [ done | ]); iSplitL ""; iFrame;
+          first done. rewrite !interp_L2_conv_tau.
+          do 2 iApply sim_coindF_tauR.
+          specialize (H4 v_s); to_eq in H4; rewrite -H4; by clear H4. } }
+
+    { to_eq in H; rewrite H; rewrite H bind_vis in H0.
+      to_eq in H0; rewrite H0.
+       iDestruct (sim_coindF_fail_inv with "He Hinner") as %Hfail.
+
+      destruct Hfail as [(?&?&Hfail) | (?&?&?)].
+
+      (* Failure *)
+      { rewrite Hfail in H1.
+        change (Tau (n_taus ?x ?n)) with (n_taus x (S n)) in H1.
+        eapply interp_L2_conv_failure_tau_n_inv in H1.
+        destruct H1 as (?&?&?).
+        to_eq in H1; rewrite H1.
+        rewrite -sim_indF_unfold.
+        iApply sim_indF_n_taus_R.
+        rewrite sim_indF_unfold /sim_expr_inner.
+        by provide_case: SOURCE_EXC. }
+
+      { rewrite H2 in H1.
+        change (Tau (n_taus ?x ?n)) with (n_taus x (S n)) in H1.
+        eapply interp_L2_conv_UB_tau_n_inv in H1.
+        destruct H1 as (?&?).
+        to_eq in H1; rewrite H1.
+        rewrite -sim_indF_unfold.
+        iApply sim_indF_n_taus_R.
+        rewrite sim_indF_unfold /sim_expr_inner.
+        by provide_case: SOURCE_UB. } }
+
+    { to_eq in H; rewrite H;  rewrite H bind_vis in H0.
+      to_eq in H0; rewrite H0.
+      iDestruct (sim_coindF_UBE_inv with "He Hinner") as %Hfail.
+
+      destruct Hfail as [(?&?&Hfail) | (?&?&?)].
+      { rewrite Hfail in H1.
+        change (Tau (n_taus ?x ?n)) with (n_taus x (S n)) in H1.
+        eapply interp_L2_conv_failure_tau_n_inv in H1.
+
+        destruct H1 as (?&?&?).
+        to_eq in H1; rewrite H1.
+        rewrite -sim_indF_unfold.
+        iApply sim_indF_n_taus_R.
+        rewrite sim_indF_unfold /sim_expr_inner.
+        by provide_case: SOURCE_EXC. }
+
+      { rewrite H2 in H1.
+        change (Tau (n_taus ?x ?n)) with (n_taus x (S n)) in H1.
+        eapply interp_L2_conv_UB_tau_n_inv in H1.
+        destruct H1 as (?&?).
+        to_eq in H1; rewrite H1.
+        rewrite -sim_indF_unfold.
+        iApply sim_indF_n_taus_R.
+        rewrite sim_indF_unfold /sim_expr_inner.
+        by provide_case: SOURCE_UB. } }
+
+    { to_eq in H; rewrite H; rewrite H bind_vis in H0.
+      setoid_rewrite bind_ret_l in H0; cbn in H0.
+      to_eq in H0; rewrite H0.
+      iDestruct "He" as "#He".
+
+      iDestruct (sim_coindF_F_inv_L with "He Hinner") as
+        ">[ Hinner | [ Hinner | Hinner ] ]".
+      { to_inner (interp_mrec_rec (R1 := T) (R2 := T)).
+        iDestruct "Hinner" as (? ? Hfail) "Hinner".
+        pose proof (Heq := Hfail).
+        rewrite -itree_eta in Hfail.
+        rewrite Hfail in H1.
+        change (Tau (n_taus ?x ?n)) with (n_taus x (S n)) in H1.
+
+        apply (interp_L2_conv_F_tau_n_inv _ _ _ _ _ g) in H1.
+        destruct H1 as (?&?&?&?&?).
+        to_eq in H3; rewrite H3.
+        rewrite -itree_eta in Heq; to_eq in Heq.
+        to_inner (interp_mrec_rec (R1 := T) (R2 := T)).
+        rewrite -sim_indF_unfold.
+        iApply sim_indF_n_taus_R.
+        rewrite sim_indF_unfold; provide_case:STUTTER_L.
+        cbn.
+        rewrite sim_indF_unfold; provide_case:VIS_STEP.
+        cbn. rewrite /handle_E.
+        iSplitL ""; first (iPureIntro; exists eq_refl; reflexivity).
+        iIntros (???). dependent destruction H3.
+        cbn; change (TauF ?x) with (observe (Tau x)).
+        rewrite -!interp_mrec_tau.
+        iLeft.
+        iExists f, _, _, g, _, _;
+          do 2 (iSplitL ""; [ done | ]); iFrame; iSplitL ""; first done.
+        iModIntro. rewrite !interp_L2_conv_tau.
+        specialize (H1 v_s); to_eq in H1; rewrite -H1.
+        do 2 iApply sim_coindF_tauL. by dependent destruction H4. }
+
+      { iDestruct "Hinner" as (?????) "Hinner".
+        rewrite -itree_eta in H3.
+        rewrite H3 in H1.
+        change (Tau (n_taus ?x ?n)) with (n_taus x (S n)) in H1.
+        eapply interp_L2_conv_UB_tau_n_inv with (g := g) in H1.
+        destruct H1 as (?&?).
+        to_eq in H1; rewrite H1.
+        to_inner (interp_mrec_rec (R1 := T) (R2 := T)).
+        rewrite -sim_indF_unfold.
+        change (Tau (n_taus ?x ?n)) with (n_taus x (S n)).
+        iApply sim_indF_n_taus_R.
+        rewrite sim_indF_unfold; by provide_case: SOURCE_UB. }
+
+      { iDestruct "Hinner" as (?????) "Hinner".
+        rewrite -itree_eta in H3.
+        rewrite H3 in H1.
+        change (Tau (n_taus ?x ?n)) with (n_taus x (S n)) in H1.
+        eapply interp_L2_conv_failure_tau_n_inv with (g := g) in H1.
+        destruct H1 as (?&?&?).
+        to_eq in H1; rewrite H1.
+        to_inner (interp_mrec_rec (R1 := T) (R2 := T)).
+        rewrite -sim_indF_unfold.
+        change (Tau (n_taus ?x ?n)) with (n_taus x (S n)).
+        iApply sim_indF_n_taus_R.
+        rewrite sim_indF_unfold; by provide_case: SOURCE_EXC. } }
+
+    Unshelve. all : eauto.
+  Qed.
+
+  Theorem Proper_interp_mrec {T}
+    (f g : ∀ T : Type, LLVMEvents.CallE T → L0'expr T) a1 a2 Ψ:
+    context_rel f g -∗
+    ⟅ a1 ⟆ ⪯ ⟅ a2 ⟆ [[ Ψ ⤉ ]] -∗
+    interp_mrec (T := T) f a1 ⪯ interp_mrec (T := T) g a2 [[ Ψ ⤉ ]].
+  Proof.
+    iIntros "H H'"; iIntros (??) "SI".
+
+    iApply (sim_coindF_strong_coind interp_mrec_pred);
+      last iApply (interp_mrec_pred_coind_init with "H H' SI"); eauto.
+
+    iModIntro. clear f g a1 a2 σ_t σ_s.
+    iIntros (Φ e_t e_s) "IH".
+    iDestruct "IH" as (????????) "(H1 & H2 & H3)"; subst.
+
+    rewrite sim_coindF_unfold.
+    iAssert (∀ Ψ e_t e_s, (sim_indF sim_coindF Ψ e_t e_s) -∗
+      interp_mrec_ind Ψ e_t e_s)%I as "Hgen"; last first.
+    { iSpecialize ("Hgen" with "H3").
+      iSpecialize ("Hgen" $! _ _ _ _ _ _ with "H1"); try done.
+      iSpecialize ("Hgen" $! eq_refl eq_refl with "H2").
+      iApply "Hgen". }
+
+    clear Φ f a1 σ_t g a2 σ_s Ψ.
+    iIntros (Ψ e_t e_s) "Hsim".
+
+    iApply (sim_indF_strong_ind with "[] Hsim"); clear Ψ e_t e_s.
+
+    iModIntro. iIntros (Ψ e_t e_s) "Hinner".
+    iIntros (??????) "#He".
+    iIntros (??) "Hr". subst.
+
+    (* [Hinner] for the "inner" expression, i.e. [e_s] *)
+    rewrite /sim_expr_inner.
+    cbn -[F] in *; rewrite sim_indF_unfold /sim_expr_inner.
+    iMod "Hinner".
+
+    to_inner (interp_mrec_rec (R1 := T) (R2 := T)).
+
+    iDestruct "Hinner" as ( c ) "Hinner";
+      destruct c; try case_solve; try done.
+
+    { (* [BASE] case *)
+      by iApply (Proper_interp_mrec_base_case with "He Hr Hinner"). }
+
+    { (* [STUTTER_L] case *)
+      by iApply (Proper_interp_mrec_stutter_l_case with "He Hr Hinner"). }
+
+    { (* [STUTTER_R] case*)
+      by iApply (Proper_interp_mrec_stutter_r_case with "He Hr Hinner"). }
+
+    { (* [TAU_STEP] case*)
+      by iApply (Proper_interp_mrec_tau_case with "He Hr Hinner"). }
+
+    { (* [VIS] case *)
+      symmetry in H0; apply simpobs in H0;
+      symmetry in H1; apply simpobs in H1.
+      pose proof (H0' := H0).
+      pose proof (H1' := H1).
+      apply interp_L2_conv_vis_inv in H0; apply interp_L2_conv_vis_inv in H1.
+
+      destruct H0 as [ (?&?&?&?&?&?) | (?&?&?&?) ];
+      destruct H1 as [ (?&?&?&?&?&?) | (?&?&?&?) ].
+      { (* Internal call *)
+        to_eq in H; to_eq in H0;
+          rewrite H H0 !interp_mrec_call.
+        rewrite H in H0'; rewrite H0 in H1'.
+        rename x into τ, x0 into addr,
+          x1 into args, x2 into attrs, x3 into k;
+        rename x4 into τ', x5 into addr',
+          x6 into args', x7 into attrs', x8 into k'.
+
+        setoid_rewrite interp_vis in H0';
+        rewrite /subevent in H0'; unfold_cat in H0'; simp L0'_conv in H0'.
+        setoid_rewrite interp_vis in H1';
+        rewrite /subevent in H1'; unfold_cat in H1'; simp L0'_conv in H1'.
+
+        rewrite bind_trigger in H0'. rewrite bind_trigger in H1'.
+        setoid_rewrite interp_state_vis in H0';
+        rewrite /subevent in H0'; unfold_cat in H0'; cbn in H0';
+          rewrite /handle_stateEff in H0'; rewrite bind_vis in H0'.
+
+        setoid_rewrite interp_state_vis in H1';
+        rewrite /subevent in H1'; unfold_cat in H1'; cbn in H1';
+          rewrite /handle_stateEff in H1'; rewrite bind_vis in H1'.
+
+        setoid_rewrite bind_ret_l in H0';
+        setoid_rewrite interp_state_tau in H0'.
+
+        setoid_rewrite bind_ret_l in H1';
+        setoid_rewrite interp_state_tau in H1'.
+
+        apply eqit_inv_Vis_weak in H0', H1'.
+        destruct H0' as (d&He&Hk); dependent destruction d.
+        destruct H1' as (d&He'&Hk'); dependent destruction d.
+        red in He; red in He'.
+        rewrite /subevent in He He'; unfold_cat in He; unfold_cat in He'.
+        subst. red in Hk, Hk'.
+
+        rewrite /handle_event. simp handle_call_events.
+
+        iDestruct "Hinner" as "[ Hinner | Hinner ]"; cycle 1.
+
+        (* Internal call was "external" and now meets the spec *)
+        { iDestruct "Hinner" as (?) "(SI & Hev & Hinner)".
+          provide_case: TAU_STEP.
+          iLeft. iDestruct "Hr" as "#Hr".
+          iExists f, _, _, g, _, _.
+          repeat (iSplitL ""; first done); iFrame.
+          iDestruct "Hr" as "(Hr_inv & _)".
+
+          (* Cut on internal call *)
+          rewrite !interp_L2_conv_bind; iApply sim_coindF_coind_bind.
+
+          iSpecialize ("Hr_inv" with "Hev SI").
+          match goal with
+            | |- environments.envs_entails _ (sim_coindF ?Φ _ _) => remember Φ
+          end.
+          setoid_rewrite sim_coindF_unfold at 3.
+          rewrite sim_indF_unfold /sim_expr_inner. iMod "Hr_inv".
+
+          to_inner (sim_coindF (R1 := uvalue) (R2 := uvalue)).
+          rewrite -sim_indF_unfold -sim_coindF_unfold.
+          iApply (sim_coindF_bupd_mono with "[Hinner]"); last done; subst.
+          iIntros (??) "HΦ".
+
+          iDestruct "HΦ" as (????) "(SI & %Ht & %Hs & HΦ)"; subst.
+          iDestruct "HΦ" as (????) "HΦ".
+          to_eq in H; to_eq in H0; rewrite H H0; cbn -[state_interp].
+          pose proof (bind_ret_l (σ_t0, v_t) (fun x => ⟦ ⟅ k x.2 ⟆ ⟧ x.1)).
+          to_eq in H1; rewrite H1; clear H1.
+          pose proof (bind_ret_l (σ_s0, v_s) (fun x => ⟦ ⟅ k' x.2 ⟆ ⟧ x.1)).
+          to_eq in H1; rewrite H1; clear H1.
+
+          cbn -[state_interp].
+          specialize (Hk (σ_t0, v_t)); specialize (Hk' (σ_s0, v_s)).
+
+          iCombine "SI HΦ" as "H"; iSpecialize ("Hinner" $! (σ_t0, v_t) (σ_s0, v_s));
+            cbn -[state_interp].
+          iSpecialize ("Hinner" with "H"); iMod "Hinner".
+          to_eq in Hk; to_eq in Hk'; rewrite -Hk -Hk'.
+
+          iPoseProof (contains_base_tauL with "He") as "#HL".
+          iPoseProof (contains_base_tauR with "He") as "#HR".
+
+          do 2 (iPoseProof (sim_coindF_TauL_inv with "HL Hinner") as "Hinner").
+          do 2 (iPoseProof (sim_coindF_TauR_inv with "HR Hinner") as "Hinner");
+          done.
+        }
+
+        { (* Calls eq *)
+          iDestruct "Hinner" as (?) "(SI & Hcall & Hinner)".
+          rewrite /call_args_eq.
+
+          Opaque arg_val_rel.
+          iDestruct "Hcall" as "(Hcall & %Hev)"; cbn in Hev; inversion Hev; subst.
+          cbn -[state_interp].
+          provide_case: TAU_STEP.
+          iLeft. iDestruct "Hr" as "#Hr".
+          iExists f, _, _, g, _, _.
+          repeat (iSplitL ""; first done).
+
+          (* Cut on internal call *)
+          rewrite !interp_L2_conv_bind; iApply sim_coindF_coind_bind.
+          iDestruct "Hr" as "(_ & Hr_refl)".
+          iSpecialize ("Hr_refl" with "Hcall SI").
+          match goal with
+            | |- environments.envs_entails _ (sim_coindF ?Φ _ _) => remember Φ
+          end.
+          setoid_rewrite sim_coindF_unfold at 3.
+          rewrite sim_indF_unfold /sim_expr_inner. iMod "Hr_refl".
+
+          to_inner (sim_coindF (R1 := uvalue) (R2 := uvalue)).
+          rewrite -sim_indF_unfold -sim_coindF_unfold.
+          iApply (sim_coindF_bupd_mono with "[Hinner]"); last done; subst.
+          iIntros (??) "HΦ".
+
+          iDestruct "HΦ" as (????) "(SI & %Ht & %Hs & HΦ)"; subst.
+          iDestruct "HΦ" as (????) "HΦ".
+          to_eq in H; to_eq in H0; rewrite H H0; cbn -[state_interp].
+          pose proof (bind_ret_l (σ_t0, v_t) (fun x => ⟦ ⟅ k x.2 ⟆ ⟧ x.1)).
+          to_eq in H1; rewrite H1; clear H1.
+          pose proof (bind_ret_l (σ_s0, v_s) (fun x => ⟦ ⟅ k' x.2 ⟆ ⟧ x.1)).
+          to_eq in H1; rewrite H1; clear H1.
+
+          cbn -[state_interp].
+          specialize (Hk (σ_t0, v_t)); specialize (Hk' (σ_s0, v_s)).
+
+          iCombine "SI HΦ" as "H"; iSpecialize ("Hinner" $! (σ_t0, v_t) (σ_s0, v_s));
+            cbn -[state_interp].
+          destruct C as (?&?).
+          iSpecialize ("Hinner" with "H"); iMod "Hinner".
+          to_eq in Hk; to_eq in Hk'; rewrite -Hk -Hk'.
+
+          iPoseProof (contains_base_tauL with "He") as "#HL".
+          iPoseProof (contains_base_tauR with "He") as "#HR".
+
+          do 2 (iPoseProof (sim_coindF_TauL_inv with "HL Hinner") as "Hinner").
+          do 2 (iPoseProof (sim_coindF_TauR_inv with "HR Hinner") as "Hinner");
+          done.
+        }
+      }
+
+      { (* Asymmetric internal-external call - absurd *)
+        to_eq in H. rewrite H in H0'.
+        setoid_rewrite interp_vis in H0'.
+        rewrite /subevent in H0'; unfold_cat in H0'.
+        simp call_conv in H0'; rewrite bind_vis in H0'.
+        setoid_rewrite interp_state_vis in H0'.
+        setoid_rewrite bind_ret_l in H0'.
+        setoid_rewrite interp_state_tau in H0'.
+        rewrite /subevent in H0'; unfold_cat in H0'.
+        cbn in H0'. rewrite /handle_stateEff in H0'.
+        rewrite bind_vis in H0'.
+
+        apply eqit_inv_Vis_weak in H0'.
+        destruct H0' as (d&He&Hk); dependent destruction d.
+        red in He; rewrite /subevent in He; unfold_cat in He.
+        subst. red in Hk.
+        rewrite /handle_event. destruct es; try done.
+
+        destruct c, p. simp handle_call_events. destruct c.
+        to_eq in H0; rewrite H0 in H1'.
+        destruct x5.
+        - setoid_rewrite interp_vis in H1'.
+          rewrite /subevent in H1'; unfold_cat in H1'.
+          rewrite /ReSum_sum /case_ /Case_sum1 /case_sum1 /resum in H1'.
+          destruct e.
+          simp call_conv in H1'. rewrite bind_vis in H1'.
+          setoid_rewrite interp_state_vis in H1'.
+          cbn in H1'. rewrite bind_vis in H1'.
+          apply eqit_inv_Vis_weak in H1'. destruct H1' as (?&?&?).
+          dependent destruction x4.
+          red in H; inversion H; subst.
+          iDestruct "Hinner" as "[ Hinner | Hinner]".
+          + iDestruct "Hinner" as (?) "(SI & Hargs & Hinner)".
+            rewrite /call_args_eq.
+            iDestruct "Hargs" as "(Hargs & %Ha)".
+            inversion Ha.
+          + iDestruct "Hinner" as (?) "(SI & Hargs & Hinner)".
+            rewrite /call_ev. iExFalso. cbn. destruct C as ((?&?)&?).
+            simp vir_call_ev.
+            iDestruct "Hargs" as "(#Hdv & Hargs)".
+            iDestruct "Hargs" as (??) "H".
+            inversion H2.
+        - setoid_rewrite interp_vis in H1'.
+          rewrite /subevent in H1'; unfold_cat in H1'.
+          rewrite /ReSum_sum /case_ /Case_sum1 /case_sum1 /resum in H1'.
+          rewrite bind_vis in H1'.
+          setoid_rewrite interp_state_vis in H1'.
+          iExFalso. iClear "Hinner".
+          destruct s0 as [ | [ | [ | [ | ] ] ] ]; cbn in H1';
+            simp call_conv in H1'; cbn in H1'.
+          all: try solve [rewrite bind_tau in H1'; by apply eqit_inv in H1'].
+          destruct s0.
+          all: try solve [rewrite bind_tau in H1'; by apply eqit_inv in H1']. }
+
+      { (* Asymmetric internal-external call *)
+        to_eq in H0. rewrite H0 in H1'.
+        setoid_rewrite interp_vis in H1'.
+        rewrite /subevent in H1'; unfold_cat in H1'.
+        simp call_conv in H1'; rewrite bind_vis in H1'.
+        setoid_rewrite interp_state_vis in H1'.
+        setoid_rewrite bind_ret_l in H1'.
+        setoid_rewrite interp_state_tau in H1'.
+        rewrite /subevent in H1'; unfold_cat in H1'.
+        cbn in H1'. rewrite /handle_stateEff in H1'.
+        rewrite bind_vis in H1'.
+
+        apply eqit_inv_Vis_weak in H1'.
+        destruct H1' as (d&He&Hk); dependent destruction d.
+        red in He; rewrite /subevent in He; unfold_cat in He.
+        subst. red in Hk.
+        rewrite /handle_event. destruct et; try destruct s; try done.
+        2 : destruct s; done.
+
+        destruct c, p. simp handle_call_events. destruct c.
+        to_eq in H; rewrite H in H0'.
+        destruct x0.
+        - setoid_rewrite interp_vis in H0'.
+          rewrite /subevent in H0'; unfold_cat in H0'.
+          rewrite /ReSum_sum /case_ /Case_sum1 /case_sum1 /resum in H0'.
+          destruct e.
+          simp call_conv in H0'. rewrite bind_vis in H0'.
+          setoid_rewrite interp_state_vis in H0'.
+          cbn in H0'. rewrite bind_vis in H0'.
+          apply eqit_inv_Vis_weak in H0'. destruct H0' as (?&?&?).
+          dependent destruction x.
+          red in H0; inversion H0; subst.
+          iDestruct "Hinner" as "[ Hinner | Hinner]".
+          + iDestruct "Hinner" as (?) "(SI & Hargs & Hinner)".
+            rewrite /call_args_eq.
+            iDestruct "Hargs" as "(Hargs & %Ha)".
+            inversion Ha.
+          + iDestruct "Hinner" as (?) "(SI & Hargs & Hinner)".
+            rewrite /call_ev. iExFalso. cbn.
+            destruct C as ((?&?)&?).
+            simp vir_call_ev.
+            iDestruct "Hargs" as "(#Hdv & Hargs)".
+            iDestruct "Hargs" as (??) "H".
+            inversion H2.
+        - setoid_rewrite interp_vis in H0'.
+          rewrite /subevent in H0'; unfold_cat in H0'.
+          rewrite /ReSum_sum /case_ /Case_sum1 /case_sum1 /resum in H0'.
+          rewrite bind_vis in H0'.
+          setoid_rewrite interp_state_vis in H0'.
+          iExFalso. iClear "Hinner".
+          destruct s0 as [ | [ | [ | [ | ] ] ] ]; cbn in H0';
+            simp call_conv in H0'; cbn in H0'.
+          all: try solve [rewrite bind_tau in H0'; by apply eqit_inv in H0'].
+          destruct s0.
+          all: try solve [rewrite bind_tau in H0'; by apply eqit_inv in H0']. }
+
+      { (* External call *)
+        to_eq in H; rewrite H in H0'; to_eq in H0; rewrite H0 in H1'.
+        pose proof (H0'' := H0').
+        apply interp_L2_conv_vis_ECall_noncall in H0'.
+        destruct H0' as (?&?&?&?&?&?&?&?).
+        cbn in *.
+        subst.
+        cbn in H0''. setoid_rewrite interp_vis in H0''.
+        rewrite /resum in H0''. unfold_cat in H0''.
+        simp L0'_conv in H0''. rewrite bind_vis in H0''.
+        setoid_rewrite interp_state_vis in H0''.
+        rewrite {1} /handle_L0_L2 in H0''.
+        cbn in H0''. rewrite /handle_stateEff in H0''.
+        rewrite bind_vis in H0''.
+        repeat setoid_rewrite bind_ret_l in H0''.
+        setoid_rewrite interp_state_tau in H0''.
+
+        apply eqit_inv in H0''. cbn in H0''. destruct H0'' as (?&?&?).
+        dependent destruction x. clear x.
+        destruct H. red in H0. rewrite /handle_event. cbn -[interp_L2].
+
+        pose proof (H1'' := H1').
+        apply interp_L2_conv_vis_ECall_noncall in H1'.
+        destruct H1' as (?&?&?&?&?&?&?&?).
+        cbn in H, H1.
+        subst.
+        cbn in H1''. setoid_rewrite interp_vis in H1''.
+        rewrite /resum in H1''. unfold_cat in H1''.
+        simp L1'_conv in H1''. rewrite bind_vis in H1''.
+        setoid_rewrite interp_state_vis in H1''.
+        rewrite {1} /handle_L0_L2 in H1''.
+        cbn in H1''. rewrite /handle_stateEff in H1''.
+        rewrite bind_vis in H1''.
+        apply eqit_inv in H1''. cbn in H1''. destruct H1'' as (?&?&?).
+        dependent destruction x2. red in H. red in H3. subst; cbn -[interp_L2].
+        rewrite /resum. unfold_cat.
+        rewrite /resum /inl_ /Inl_sum1.
+
+        rewrite !interp_mrec_external_call.
+        provide_case: VIS_STEP. rewrite /subevent /resum /ReSum_inl /cat; unfold_cat.
+        rewrite /inl_ /Inl_sum1.
+        rewrite /handle_event. rewrite /Id_IFun.
+
+        simp handle_call_events.
+        iDestruct "Hinner" as "[ Hinner |  Hinner ]".
+        { iDestruct "Hinner" as (?) "(SI & Hargs & Hk)".
+          iLeft. iFrame.
+          rewrite /call_args_eq.
+          iDestruct "Hargs" as "(Hargs & %Hargs)".
+          inversion Hargs; subst; iFrame.
+          iExists _; iFrame.
+          iSplitL ""; first (iPureIntro; eauto).
+          iIntros (??) "H".
+          iSpecialize ("Hk" with "H").
+          iMod "Hk". rewrite -!interp_mrec_tau. iLeft.
+          iExists f, _, _, g, _, _; iFrame.
+          repeat (iSplitL ""; first done).
+          rewrite !interp_L2_conv_tau.
+          specialize (H0 (v_t.1, call_returns (ExternalCall x2 x6 x7 x10) v_t.2)).
+          to_eq in H0; rewrite -H0.
+          specialize (H3 (v_s.1, call_returns (ExternalCall x2 x6 x7 x10) v_s.2)).
+          repeat rewrite bind_ret_l in H3.
+          rewrite interp_state_tau in H3. to_eq in H3. rewrite -H3. done. }
+
+        { iDestruct "Hinner" as (?) "(SI & Hargs & Hk)".
+          iRight. iFrame.
+          rewrite /call_ev.
+          cbn -[state_interp].
+          destruct C as ((?&?)&?).
+          simp vir_call_ev.
+          iDestruct "Hargs" as "(#Hdv & Hargs)".
+          iDestruct "Hargs" as (??) "(#Hv & HC & #HWF & Hst & Hss & %Hinterp)".
+          subst; iFrame.
+          iExists (g0, l, l0).
+          iSplitL "Hst Hss HC".
+          { simp vir_call_ev. iFrame. inversion H4; subst; eauto.
+            repeat (iSplitL ""; first done). done. }
+
+          iIntros (??) "H".
+          iDestruct "H" as "(SI & H)".
+          iPoseProof (vir_call_ans_attr with "H") as "H".
+          iCombine "SI H" as "H".
+          change (TauF ?x) with (observe (Tau x)).
+
+          iSpecialize ("Hk" with "H").
+          iMod "Hk". rewrite -!interp_mrec_tau. iLeft.
+          iExists f, _, _, g, _, _; iFrame.
+          repeat (iSplitL ""; first done).
+          rewrite !interp_L2_conv_tau.
+          specialize (H0 v_t).
+          to_eq in H0; rewrite -H0.
+          specialize (H3 v_s).
+          repeat rewrite bind_ret_l in H3.
+          rewrite interp_state_tau in H3. to_eq in H3. rewrite -H3. done. } } }
+
+    { (* [UB] case *)
+      inversion Heq.
+      symmetry in H0; apply simpobs in H0.
+      by eapply interp_L2_conv_UB_inv in H0. }
+
+    { (* [EXC] case *)
+      inversion Heq.
+      symmetry in H0; apply simpobs in H0.
+      by eapply interp_L2_conv_failure_inv in H0. }
+  Qed.
+
+  Definition inv i_t i_s :=
+    (frame_WF i_t i_s ∗ checkout ∅ ∗ stack_tgt i_t ∗ stack_src i_s)%I.
+
+  Theorem Proper_interp_mrec' {R}
+    (f g : ∀ T : Type, LLVMEvents.CallE T → L0'expr T) a1 a2
+    (Ψ : R -d> R -d> iPropI Σ) i_t i_s :
+    inv i_t i_s -∗
+    context_rel f g -∗
+    <pers>
+      (inv i_t i_s -∗ ⟅ a1 ⟆ ⪯ ⟅ a2 ⟆ [[ (fun x y => Ψ x y ∗ inv i_t i_s) ⤉ ]]) -∗
+    interp_mrec f a1 ⪯ interp_mrec g a2
+    [[ (fun x y => Ψ x y ∗ inv i_t i_s) ⤉ ]].
+  Proof.
+    iIntros "Hinv Hrel #Hr".
+    iSpecialize ("Hr" with "Hinv").
+    iApply (Proper_interp_mrec with "Hrel Hr").
+  Qed.
+
+  Lemma sim_pick_unique_args args1 args2:
+    ⊢ ([∗ list] x;y ∈ args1;args2, uval_rel x y) -∗
+    ⟅ map_monad (λ uv : uvalue, pickUnique uv) args1 ⟆ ⪯
+    ⟅ map_monad (λ uv : uvalue, pickUnique uv) args2 ⟆
+    [[ (fun r1 r2 =>
+          ([∗ list] d; u ∈ r1; args1, ⌜determine_uvalue u d⌝) ∗
+          ([∗ list] d; u ∈ r2; args2, ⌜determine_uvalue u d⌝)) ⤉ ]].
+  Proof.
+    iIntros "#Hl".
+    iInduction args2 as [ | ] "IH" forall (args1).
+    { iDestruct (big_sepL2_nil_inv_r with "Hl") as %Hargs1; subst; cbn.
+      setoid_rewrite interp_ret. iApply sim_expr'_base.
+      iExists _, _; repeat (iSplitL ""; first done); done. }
+
+    { iDestruct (big_sepL2_cons_inv_r with "Hl") as (???) "(Ha & Hl')";
+        subst; cbn.
+      setoid_rewrite interp_bind.
+      rewrite {3 5} /pickUnique.
+
+      iApply sim_expr'_bind.
+      iPoseProof (L0_conv_concretize_or_pick_strong with "Ha") as "H".
+      iApply sim_expr'_bupd_mono; cycle 1.
+      { iApply sim_expr_lift; rewrite /instr_conv; iApply "H". }
+      iIntros (??) "H'".
+      iDestruct "H'" as (????) "(Hd & %Ht & %Hs)".
+      rewrite H H0; rewrite !bind_ret_l; clear H H0.
+      rewrite !interp_bind.
+
+      iApply sim_expr'_bind; iModIntro.
+      iApply sim_expr'_bupd_mono; [ | iApply ("IH" with "Hl'")].
+
+      clear e_t0 e_s0. iClear "H".
+      iIntros (??); iIntros "H".
+      iDestruct "H" as (????) "(H1 & H2)".
+      rewrite H H0 !bind_ret_l !interp_ret.
+      iApply sim_expr'_base. iModIntro; iExists _, _.
+      do 2 (iSplitL ""; first done); cbn; iFrame.
+      iSplitL ""; done. }
+  Qed.
+
+  Lemma determine_uvalue_uval_rel uv1 dv1 uv2 dv2:
+    determine_uvalue uv1 dv1 ->
+    determine_uvalue uv2 dv2 ->
+    uval_rel uv1 uv2 -∗
+    uval_rel (dv1 ̂) (dv2 ̂).
+  Proof.
+    rewrite /determine_uvalue.
+    iIntros (Hd1 Hd2) "#Hr".
+    destruct (is_concrete uv1) eqn: Hv1.
+    { apply uvalue_to_dvalue_inv in Hd1; subst.
+      destruct (is_concrete uv2) eqn: Hv2.
+      { by apply uvalue_to_dvalue_inv in Hd2; subst. }
+      { iSpecialize ("Hr" $! _ Hd2).
+        iDestruct "Hr" as (??) "Hr".
+        iIntros (??).
+        rewrite !concretize_uvalue_dvalue_to_uvalue in H, H0.
+        inversion H; inversion H0; subst.
+        rewrite concretize_uvalue_dvalue_to_uvalue.
+        iExists _; iSplitL ""; done. } }
+    { destruct (is_concrete uv2) eqn: Hv2.
+      { apply uvalue_to_dvalue_inv in Hd2; subst.
+        iIntros (??).
+        rewrite !concretize_uvalue_dvalue_to_uvalue in H;
+          inversion H; subst.
+        rewrite /uval_rel.
+        rewrite !concretize_uvalue_dvalue_to_uvalue.
+        iSpecialize ("Hr" $! _ eq_refl).
+        iDestruct "Hr" as (??) "Hv".
+        iExists _; iSplitL ""; first done.
+        clear H Hv2. rewrite Hd1 in H0; inversion H0; by subst. }
+      { iSpecialize ("Hr" $! _ Hd2).
+        iDestruct "Hr" as (??) "Hr".
+        iIntros (??).
+        rewrite !concretize_uvalue_dvalue_to_uvalue in H, H0.
+        inversion H; inversion H0; subst.
+        rewrite concretize_uvalue_dvalue_to_uvalue.
+        iExists _; iSplitL ""; first done. clear H2.
+        rewrite Hd1 in H; inversion H; by subst. } }
+  Qed.
+
+  Lemma uval_rel_determine_uvalue_dvalue_to_uvalue args_t args_s v_t v_s :
+    ([∗ list] x;y ∈ args_t;args_s, uval_rel x y) -∗
+    ([∗ list] d;u ∈ v_t;args_t, ⌜determine_uvalue u d⌝) -∗
+    ([∗ list] d;u ∈ v_s;args_s, ⌜determine_uvalue u d⌝) -∗
+    ([∗ list] x;y ∈ map dvalue_to_uvalue v_t;map dvalue_to_uvalue v_s,
+       uval_rel x y).
+  Proof.
+    iIntros "#HR".
+    iInduction args_t as [ | ] "IH" forall (args_s v_t v_s).
+    { iIntros "#H_t #H_s".
+      iDestruct (big_sepL2_nil_inv_l with "HR") as %Hr; subst.
+      iDestruct (big_sepL2_nil_inv_r with "H_t") as %Hr; subst.
+      iDestruct (big_sepL2_nil_inv_r with "H_s") as %Hr; subst.
+      done. }
+    { iDestruct (big_sepL2_cons_inv_l with "HR") as (???) "(Hr & Hl)".
+      iIntros "#H_t #H_s".
+      iDestruct (big_sepL2_cons_inv_r with "H_t") as (????) "H_t'"; subst.
+      iDestruct (big_sepL2_cons_inv_r with "H_s") as (????) "H_s'"; subst.
+      cbn.
+      iPoseProof (determine_uvalue_uval_rel _ _ _ _ H1 H0 with "Hr") as "Hd".
+      iSplitL ""; first done.
+      by iSpecialize ("IH" with "Hl H_t' H_s'"). }
+  Qed.
+
+  Lemma sim_external_call dτ addr_t addr_s args_t args_s l i_t i_s:
+    frame_WF i_t i_s -∗
+    stack_tgt i_t -∗
+    stack_src i_s -∗
+    checkout ∅ -∗
+    dval_rel addr_t addr_s -∗
+    ([∗ list] x;y ∈ args_t;args_s, uval_rel x y) -∗
+    ⟅ dargs <- map_monad (λ uv : uvalue, pickUnique uv) args_t;;
+      trigger (ExternalCall dτ addr_t (map dvalue_to_uvalue dargs) l) ⟆
+    ⪯
+    ⟅ dargs <- map_monad (λ uv : uvalue, pickUnique uv) args_s;;
+      trigger (ExternalCall dτ addr_s (map dvalue_to_uvalue dargs) l) ⟆
+    [[ (fun x y =>
+          uval_rel x y ∗ stack_tgt i_t ∗ stack_src i_s ∗
+          checkout ∅) ⤉ ]].
+  Proof.
+    iIntros "#WF Hs_t Hs_s HC #Haddr #Hargs".
+    setoid_rewrite interp_bind.
+    iApply sim_expr'_bind.
+    iApply (sim_expr'_bupd_mono with "[Hs_t Hs_s HC]");
+      last iApply (sim_pick_unique_args with "Hargs").
+    iIntros (??) "H".
+    iDestruct "H" as (????) "(#H_t & #H_s)".
+    rewrite H H0 !bind_ret_l; clear H H0.
+    rewrite !interp_vis; cbn.
+    setoid_rewrite interp_ret; cbn.
+    rewrite /subevent; unfold_cat; simp L0'_conv.
+    rewrite !bind_vis.
+    setoid_rewrite bind_ret_l.
+
+    iModIntro. simp call_conv.
+    iIntros (??) "SI"; iModIntro.
+    setoid_rewrite interp_state_vis; cbn -[state_interp].
+    rewrite /handle_stateEff !bind_vis.
+    rewrite /sim_coind' sim_coindF_unfold sim_indF_unfold.
+
+    provide_case: VIS_STEP.
+    rewrite /handle_event; cbn -[state_interp]; unfold_cat.
+    simp handle_call_events; cbn -[state_interp]. iFrame.
+    iLeft; iExists (∅, i_t, i_s).
+    Transparent arg_val_rel.
+    rewrite /call_args_eq; rewrite /arg_val_rel; cbn. iFrame. iSplitL "Haddr".
+    { rewrite /call_args_eq; cbn; iFrame.
+      iSplitL ""; last done.
+      rewrite /arg_val_rel; cbn.
+      iFrame "WF".
+
+      iSplitL ""; first done.
+      iApply (uval_rel_determine_uvalue_dvalue_to_uvalue with
+                "Hargs H_t H_s"). }
+
+    iIntros (??) "(SI & UV)".
+    iApply sim_coindF_tau; cbn -[state_interp].
+    iApply sim_coindF_tau; cbn -[state_interp].
+    iApply sim_coindF_base.
+    iExists _, _, (Ret _), (Ret _); iFrame.
+    iSplitL "".
+    { iPureIntro.
+      change (RetF (E := language.L2 vir_lang) ?x) with
+        (observe (E := language.L2 vir_lang) (Ret x)).
+      f_equiv. constructor. f_equiv. to_eq;
+        by setoid_rewrite interp_state_ret. }
+    iSplitL "".
+    { iPureIntro.
+      change (RetF (E := language.L2 vir_lang) ?x) with
+        (observe (E := language.L2 vir_lang) (Ret x)).
+      f_equiv. constructor. f_equiv. to_eq;
+        by setoid_rewrite interp_state_ret. }
+
+    iExists _, _. iDestruct "UV" as "(?&?&?&?)"; iFrame.
+    by repeat (iSplitL ""; first done).
+  Qed.
+
+End CR.
