theories/vir/toplevel.v
@@ -1,0 +1,103 @@
+
+From velliris.logic Require Import satisfiable.
+From velliris.program_logic Require Import program_logic.
+From velliris.vir Require Import
+  vir val_rel heapbij adequacy spec globalbij logical_relations fundamental
+  contextual_mcfg.
+
+From Vellvm Require Import Syntax.DynamicTypes Handlers Syntax.LLVMAst
+  Semantics.InterpretationStack Utils.Util.
+
+From ITree Require Import ITree Eq.
+
+Require Import LLVMEvents.
+Require Import CFG.
+
+(* ------------------------------------------------------------------------ *)
+
+(** *Top-level denotation *)
+(* Note: This definition is temporarily living here as a duplicate of
+ [Semantics/TopLevel.v] from Vellvm due to universe inconsistencies. *)
+
+Definition initialize_global (g:global dtyp) : itree exp_E unit :=
+  let dt := (g_typ g) in
+  a <- trigger (GlobalRead (g_ident g));;
+  uv <- match (g_exp g) with
+       | None => Monad.ret (UVALUE_Undef dt)
+       | Some e =>  denote_exp (Some dt) e
+       end ;;
+  dv <- concretize_or_pick uv True ;;
+  trigger (Store a dv).
+
+Definition initialize_globals (gs:list (global dtyp)): itree exp_E unit :=
+  map_monad_ initialize_global gs.
+
+Definition allocate_global (g:global dtyp) : itree L0 unit :=
+  ITree.bind (trigger (Alloca (g_typ g)))
+  (fun v => trigger (GlobalWrite (g_ident g) v)).
+
+Definition allocate_globals (gs:list (global dtyp)) : itree L0 unit :=
+  map_monad_ allocate_global gs.
+
+(* Returns `true` only if both function are named and have
+     the same name.
+ *)
+Definition function_name_eq (a b:function_id) : bool :=
+  match a, b with
+  | Name aname, Name bname => String.eqb aname bname
+  | _, _ => false
+  end.
+
+Definition allocate_declaration (d:declaration dtyp) : itree L0 unit :=
+  match List.find (fun x => function_name_eq (dc_name d) (dc_name x))
+          IntrinsicsDefinitions.defined_intrinsics_decls with
+  | Some _ => Ret tt (* Don't allocate pointers for LLVM intrinsics declarations *)
+  | None =>
+    ITree.bind (trigger (Alloca DTYPE_Pointer))
+    (fun v => trigger (GlobalWrite (dc_name d) v))
+  end.
+
+Definition allocate_declarations (ds:list (declaration dtyp)) : itree L0 unit :=
+  map_monad_ allocate_declaration ds.
+
+Definition build_global_environment (CFG : CFG.mcfg dtyp) : itree L0 unit :=
+  ITree.bind (allocate_declarations ((m_declarations CFG) ++ (List.map (df_prototype) (m_definitions CFG))))
+  (fun _ => ITree.bind (allocate_globals (m_globals CFG))
+  (fun _ => translate exp_to_L0 (initialize_globals (m_globals CFG)))).
+
+Definition denote_vellvm
+           (ret_typ : dtyp)
+           (entry : string)
+           (args : list uvalue)
+           (mcfg : CFG.mcfg dtyp) : itree L0 uvalue :=
+  ITree.bind (build_global_environment mcfg)
+  (fun _=>
+   ITree.bind (Util.map_monad address_one_function (m_definitions mcfg))
+    (fun defns =>
+       ITree.bind (trigger (GlobalRead (Name entry)))
+          (fun addr => denote_mcfg defns ret_typ addr args))).
+
+Import ListNotations.
+
+Definition main_args :=
+  DV.UVALUE_I64 (DynamicValues.Int64.zero) ::
+   DV.UVALUE_Addr (Addr.null) :: nil.
+
+Definition denote_vellvm_main (mcfg : CFG.mcfg dtyp) : itree L0 uvalue :=
+  denote_vellvm (DTYPE_I (32)%N) "main" main_args mcfg.
+
+(* ------------------------------------------------------------------------ *)
+
+(** Properties about the top-level denotation *)
+Section toplevel.
+
+  Context `(sheapGS Σ, checkedoutGS Σ, heapbijGS Σ).
+
+  Lemma denote_vellvm_main_global C_t C_s Φ :
+    ⊢ denote_vellvm_main C_t ⪯ denote_vellvm_main C_s [[ Φ ]].
+  Proof.
+    rewrite /denote_vellvm_main /denote_vellvm.
+
+End toplevel.
+
+(* ------------------------------------------------------------------------ *)
