theories/program_logic/simulation.v
@@ -26,9 +26,9 @@ Class SimE (PROP : bi) (Λ : language) :=
 (* FIXME what are good levels for et, es? *)
 
 Notation "et '⪯' es ⦃ Φ ⦄" := (sim Φ et es) (at level 70, Φ at level 200,
-  format "'[hv' et  '/' '⪯' '/' es  '/' ⦃   Φ  ⦄ ']'") : bi_scope.
+  format "'[hv' et  '/' '⪯'  '/' es  '/' ⦃   Φ  ⦄ ']'") : bi_scope.
 Notation "et '⪯' es {{ Φ }}" := (simV Φ et es) (at level 70, Φ at level 200,
-  format "'[hv' et  '/' '⪯' '/' es  '/' {{  '[ ' Φ  ']' }} ']'") : bi_scope.
+  format "'[hv' et  '/' '⪯'  '/' es  '/' {{  '[ ' Φ  ']' }} ']'") : bi_scope.
 
 (* FIXME: the notation with binder doesn't work; left-factoring seems to fail.
 notation "et  '⪯'  es  {{  v_t  v_s ,  p  }}" := (sim et es (λ v_t v_s, p)) (at level 40, v_t, v_s at level 200, p at level 200) : bi_scope. *)
@@ -39,4 +39,4 @@ Notation "et '⪯' es [{ Φ }]" := (sim_expr Φ et es) (at level 70, Φ at level
 Notation "et '⪯' es [{ ( x ,  y  ) , Q }]" :=
   (sim_expr (fun e_t e_s => (∃ x y, ⌜e_t ≅ Ret x⌝ ∗ ⌜e_s ≅ Ret y⌝ ∗ Q)%I) et es)
     (at level 70, Q at level 200,
-      format "'[hv' et  '/' '⪯' '/' es  '/' [{  '[ ' ( x ,  y ) , '/' Q ']' }] ']'") : bi_scope.
+      format "'[hv' et  '/' '⪯'  '/' es  '/' [{  '[ ' ( x ,  y ) , '/' Q ']' }] ']'") : bi_scope.
